Add Tree Validation test vector

fstar/test/MLS_Test_Reader.ml
@@ -23,6 +23,11 @@ let int_to_uint64 (x:int): FStar_UInt64.t =
   else
     failwith "int_to_uint64: number of out bounds"
 
+let parse_string (json:Yojson.Safe.t): string =
+  match json with
+  | `String x -> x
+  | _ -> failwith "parse_string: not a string"
+
 let parse_uint32 (json:Yojson.Safe.t): FStar_UInt32.t =
   match json with
   | `Int x -> int_to_uint32 x
@@ -406,6 +411,26 @@ let parse_welcome_test (json:Yojson.Safe.t): welcome_test =
     }
   | _ -> failwith "parse_welcome_test: incorrect test vector format"
 
+(*** Tree Validation ***)
+
+let parse_tree_validation_test (json:Yojson.Safe.t): tree_validation_test =
+  match json with
+  | `Assoc [
+    ("cipher_suite", `Int cipher_suite);
+    ("group_id", `String group_id);
+    ("resolutions", `List resolutions);
+    ("tree", `String tree);
+    ("tree_hashes", `List tree_hashes);
+  ] ->
+    {
+      cipher_suite6 = int_to_uint16 cipher_suite;
+      tree = tree;
+      group_id2 = group_id;
+      resolutions = List.map (map_json parse_uint32) resolutions;
+      tree_hashes = List.map parse_string tree_hashes;
+    }
+  | _ -> failwith "parse_tree_validation_test: incorrect test vector format"
+
 (*** Messages ***)
 
 let parse_messages_test (json:Yojson.Safe.t): messages_test =
@@ -470,8 +495,8 @@ let parse_commit_transcript_test (json:Yojson.Safe.t): commit_transcript_test =
     ("tree_hash_before", `String tree_hash_before);
   ] ->
     ({
-      cipher_suite6 = int_to_uint16 cipher_suite;
-      group_id2 = group_id;
+      cipher_suite7 = int_to_uint16 cipher_suite;
+      group_id3 = group_id;
       epoch1 = parse_uint64 epoch;
       tree_hash_before = tree_hash_before;
       confirmed_transcript_hash_before = confirmed_transcript_hash_before;
@@ -505,7 +530,7 @@ let parse_treekem_test (json:Yojson.Safe.t): treekem_test =
     ("update_sender", `Int update_sender);
   ] ->
     ({
-      cipher_suite7 = int_to_uint16 cipher_suite;
+      cipher_suite8 = int_to_uint16 cipher_suite;
       input = {
         ratchet_tree_before = ratchet_tree_before;
         add_sender = int_to_uint32 add_sender;
@@ -537,6 +562,7 @@ let get_filename (typ:test_type): string =
   | KeySchedule -> "test_vectors/data/key-schedule.json"
   | PreSharedKeys -> "test_vectors/data/psk_secret.json"
   | Welcome -> "test_vectors/data/welcome.json"
+  | TreeValidation -> "test_vectors/data/tree-validation.json"
   | Messages -> "test_vectors/data/messages.json"
   | CommitTranscript -> "test_vectors/data/commit_transcript.json"
   | TreeKEM -> "test_vectors/data/treekem.json"
@@ -592,6 +618,12 @@ let get_testsuite (typ:test_type): testsuite =
     match json with
     | `List l ->
       (Welcome_test (List.map parse_welcome_test l))
+    | _ -> failwith "get_testsuite: incorrect test vector format"
+  end
+  | TreeValidation -> begin
+    match json with
+    | `List l ->
+      (TreeValidation_test (List.map parse_tree_validation_test l))
     | _ -> failwith "get_testsuite: incorrect test vector format"
   end
   | Messages -> begin
